src/defs/statics.lean
@@ -25,3 +25,17 @@ inductive has_typ: cx typ -> exp -> typ -> Prop
     has_typ Γ e1 (typ.arrow τ1 τ2) ->
     has_typ Γ e2 τ1 ->
     has_typ Γ (exp.app e1 e2) τ2
+| unit {Γ: cx typ}: has_typ Γ exp.unit typ.unit
+| prod
+    {Γ: cx typ} {e1 e2: exp} {τ1 τ2: typ}:
+    has_typ Γ e1 τ1 ->
+    has_typ Γ e2 τ2 ->
+    has_typ Γ (exp.prod e1 e2) (typ.prod τ1 τ2)
+| prod_left
+    {Γ: cx typ} {e: exp} {τ1 τ2: typ}:
+    has_typ Γ e (typ.prod τ1 τ2) ->
+    has_typ Γ (exp.prod_left e) τ1
+| prod_right
+    {Γ: cx typ} {e: exp} {τ1 τ2: typ}:
+    has_typ Γ e (typ.prod τ1 τ2) ->
+    has_typ Γ (exp.prod_right e) τ2
