src/defs/syntax.lean
@@ -6,6 +6,8 @@ inductive typ: Type
 | int: typ
 | bool: typ
 | arrow: typ -> typ -> typ
+| unit: typ
+| prod: typ -> typ -> typ
 
 -- expressions
 inductive exp: Type
@@ -16,3 +18,7 @@ inductive exp: Type
 | var: var -> exp
 | fn: var -> typ -> exp -> exp
 | app: exp -> exp -> exp
+| unit: exp
+| prod: exp -> exp -> exp
+| prod_left: exp -> exp
+| prod_right: exp -> exp
