src/lemmas/fv.lean
@@ -14,6 +14,18 @@ theorem fn_fv (x: var) (τ: typ) (e: exp):
   fv (exp.fn x τ e) = list.filter (ne x) (fv e)
   := by simp [fv]
 
+theorem prod_fv (e1 e2: exp):
+  fv (exp.prod e1 e2) = fv e1 ++ fv e2
+  := by simp [fv]
+
+theorem prod_left_fv (e: exp):
+  fv (exp.prod_left e) = fv e
+  := by simp [fv]
+
+theorem prod_right_fv (e: exp):
+  fv (exp.prod_right e) = fv e
+  := by simp [fv]
+
 theorem if_fv_empty
   (e1 e2 e3: exp)
   : fv (exp.if_ e1 e2 e3) = [] ↔ (fv e1 = [] ∧ fv e2 = [] ∧ fv e3 = []) :=
@@ -46,6 +58,22 @@ begin
   intro h,
   cases h,
   rw app_fv e1 e2 at *,
+  rw h_left,
+  rw h_right,
+  simp [list.append],
+end
+
+theorem prod_fv_empty
+  (e1 e2: exp)
+  : fv (exp.prod e1 e2) = [] ↔ (fv e1 = [] ∧ fv e2 = []) :=
+begin
+  split,
+  intro h,
+  rw prod_fv e1 e2 at h,
+  exact iff.elim_left (append_nil_both (fv e1) (fv e2)) h,
+  intro h,
+  cases h,
+  rw prod_fv e1 e2 at *,
   rw h_left,
   rw h_right,
   simp [list.append],
