src/lemmas/inversion.lean
@@ -36,3 +36,37 @@ begin
   refl,
   exact et_a,
 end
+
+theorem inversion_prod
+  {Γ: cx typ} {e1 e2: exp} {τ: typ}
+  (et: has_typ Γ (exp.prod e1 e2) τ)
+  : ∃ (τ1 τ2: typ), τ = (typ.prod τ1 τ2) ∧ has_typ Γ e1 τ1 ∧ has_typ Γ e2 τ2 :=
+begin
+  cases et,
+  existsi [et_τ1, et_τ2],
+  split,
+  refl,
+  split,
+  exact et_a,
+  exact et_a_1,
+end
+
+theorem inversion_prod_left
+  {Γ: cx typ} {e: exp} {τ1: typ}
+  (et: has_typ Γ (exp.prod_left e) τ1)
+  : ∃ (τ2: typ), has_typ Γ e (typ.prod τ1 τ2) :=
+begin
+  cases et,
+  existsi et_τ2,
+  exact et_a,
+end
+
+theorem inversion_prod_right
+  {Γ: cx typ} {e: exp} {τ2: typ}
+  (et: has_typ Γ (exp.prod_right e) τ2)
+  : ∃ (τ1: typ), has_typ Γ e (typ.prod τ1 τ2) :=
+begin
+  cases et,
+  existsi et_τ1,
+  exact et_a,
+end
